\documentclass{article}
\usepackage{cancel}
\title{Astro HW 1}
\author{Pierson Lipschultz}

\begin{document}
\maketitle
\section{}
\subsection{}
\begin{itemize}
    \item A) Collaboration and working with fellow students is encouraged, however, work still must be that of the individual, and copying answers is not allowed 
    \item B) Copying from others, cheating, enabling others to cheat, all are violations of academic honesty
    \item C) Because they are the words/work of someone other than myself
\end{itemize}
\subsection{}

\[tan^{-1}(\frac{61}{384}) \approx 9.0\deg\] \\
\[9.0 * \frac{\pi}{180} \approx .16rad\]4

\subsection{}

\[G = 6.67430 * 10^{-11} m^{3} kg^{-1} s^{-2} = 39.5 AU^{3} M_{\odot}^{-1} yr^{-2}\]

\[6.67430 * 10^{-11} m^{3} kg^{-1} s^{-2} * 1.989 * 10^{30}kg M_{\odot}\]

\[6.67430 * 10^{-11} m^{3} \cancel{kg^{-1}} s^{-2} * 1.989 * 10^{30}\cancel{kg} M_{\odot}\]

\[6.67430 * 10^{-11} m^{3} s^{-2} * 1.989 * 10^{30} M_{\odot} * {(1.496 * 10^{11})}^3 AU^3 m^{-3}\]

\[6.67430 * 10^{-11} \cancel{m^{3}} s^{-2} * 1.989 * 10^{30} M_{\odot} * {(1.496 * 10^{11})}^3 AU^3 \cancel{m^{-3}}\]

\[6.67430 * 10^{-11} s^{-2} * 1.989 * 10^{30} M_{\odot} * {(1.496 * 10^{11})}^3 AU^3 * {(3.154 * 10^7)}^2 s^{2} y^{-2}\] 

\[6.67430 * 10^{-11} \cancel{s^{-2}} * 1.989 * 10^{30} M_{\odot} * {(1.496 * 10^{11})}^3 AU^3 * {(3.154 * 10^7)}^2 \cancel{s^{2}} y^{-2}\] 

\[6.67430 * 10^{-11} * 1.989 * 10^{30} M_{\odot} * {(1.496 * 10^{11})}^3 AU^3 * {(3.154 * 10^7)}^2 y^{-2}\] 

\[ = 39.5 AU^{3} M_{\odot}^{-1} yr^{-2}\]

\subsection{}

\subsubsection{a}

\[\frac{x}{\hat{s}} = \cos(\delta)\]
\[x = \cos(\delta)\]
\[x = \hat{x}\cos(\delta)\]

\[\frac{z}{\hat{s}} = \sin(\delta)\]
\[z = \sin(\delta)\]
\[z = \hat{z}\sin(\delta)\]

\[\hat{s} = \hat{x}\cos(\delta) + \hat{z}\sin(\delta) \]

\subsubsection{b}

\[\frac{z'}{\hat{x}} = \cos(\ell)\]
\[z' = \cos(\ell)\]
\[z' = \hat{z'}\cos(\ell)\]

\[\frac{x}{\hat{x}} = \sin(\ell)\]
\[x' = \sin(\ell)\]
\[x' = \hat{x'}\sin(\ell)\]

\[\hat{x} = \hat{z'}\cos(\ell) + \hat{x'}\sin(\ell)\]

\subsubsection{c}

\[\frac{z'}{\hat{z}} = \cos(90 - \ell)\]
\[z' = \cos(90 - \ell)\]
\[z' = \hat{z'}\cos(90 - \ell)\]

\[\frac{-x'}{\hat{z}} = \sin(90 - \ell)\]
\[-x' = \sin(90 - \ell)\]
\[-x' = \hat{x'}\sin(90 - \ell)\]

\[\hat{z} = \hat{z'}\cos(90 - \ell) - \hat{x'}\sin(90 - \ell)\]

\subsubsection{d}

\[\hat{s} = \hat{x}\cos(\ell) + \hat{z}\sin(\ell) \]

\[\hat{s} = (\hat{z'}\cos(\ell) + \hat{x'}\sin(\ell))\cos(\ell) + (\hat{z'}\cos(90 - \ell) - \hat{x'}\sin(90 - \ell))\sin(\ell)\]

\[\hat{s} = \cos(\ell)(\hat{z'}\cos(\ell) + \hat{x'}\sin(\ell)) + \sin(\ell)(\hat{z'}\cos(90 - \ell) - \hat{x'}\sin(90 - \ell))\]

\subsubsection{e}

\[\theta = \ell + \delta, \ell < \delta\]

\[\theta = \ell - \delta, \ell > \delta\]

\subsubsection{f}

\subsubsection{g}

\subsubsection{h}
\[\delta = \ell\]

\end{document}